Implement necessary instances for hashing

Tables/DataType.lean
@@ -1,26 +1,30 @@
 module
 
+import Std.Data.HashMap
+
+public section
+
 namespace String
 
-public def joinSep (sep : String) (xs : Array String) : String :=
+def joinSep (sep : String) (xs : Array String) : String :=
   xs.foldl (fun acc x => if acc.isEmpty then x else acc ++ sep ++ x) ""
 
 end String
 
 namespace Tables
 
-public inductive DataType where
+inductive DataType where
   | bool
   | nat
   | string
   | option (dt : DataType)
   | array (dt : DataType)
-deriving Repr, Ord, DecidableEq
+deriving Repr, DecidableEq, Hashable
 
 namespace DataType
 
 @[expose, reducible]
-public def toType (dt : DataType) : Type :=
+def toType (dt : DataType) : Type :=
   match dt with
   | bool => Bool
   | nat => Nat
@@ -28,7 +32,7 @@ public def toType (dt : DataType) : Type :=
   | option dt => Option (toType dt)
   | array dt => Array (toType dt)
 
-public def toString (dt : DataType) (x : dt.toType) : String :=
+def toString (dt : DataType) (x : dt.toType) : String :=
   match dt with
   | bool => ToString.toString x
   | nat => ToString.toString x
@@ -39,6 +43,79 @@ public def toString (dt : DataType) (x : dt.toType) : String :=
     | none => "none"
   | array dt => s!"#[{x.map (toString dt) |> String.joinSep ", "}]"
 
+def beq (dt : DataType) (x y : dt.toType) : Bool :=
+  match dt with
+  | bool => x == y
+  | nat => x == y
+  | string => x == y
+  | option dt =>
+    match x, y with
+    | some x, some y => beq dt x y
+    | some x, none => false
+    | none, some y => false
+    | none, none => true
+  | array dt =>
+    if h : x.size = y.size then
+      Nat.all x.size fun i isLt => beq dt x[i] y[i]
+    else
+      false
+
+theorem beq_refl {dt : DataType} {x : dt.toType} : beq dt x x := by
+  induction dt with
+  | bool => grind [beq]
+  | nat => grind [beq]
+  | string => grind [beq]
+  | option dt ih =>
+    simp only [beq]
+    split <;> grind
+  | array dt ih => grind [beq]
+
+theorem eq_of_beq {dt : DataType} {x y : dt.toType} (h : beq dt x y) : x = y := by
+  induction dt with
+  | bool => grind [beq]
+  | nat => grind [beq]
+  | string => grind [beq]
+  | option dt ih =>
+    simp only [beq] at h
+    split at h <;> grind
+  | array dt ih =>
+    simp only [beq] at h
+    split at h
+    next h' =>
+      simp only [Nat.all_eq_finRange_all, List.all_eq_true, List.mem_finRange, forall_const] at h
+      refine Array.ext h' fun i hi₁ hi₂ => ?_
+      exact ih (h ⟨i, hi₁⟩)
+    next => contradiction
+
+instance {dt : DataType} : BEq dt.toType where
+  beq := beq dt
+
+instance {dt : DataType} : LawfulBEq dt.toType where
+  rfl := beq_refl
+  eq_of_beq := eq_of_beq
+
+instance {dt : DataType} : DecidableEq dt.toType :=
+  instDecidableEqOfLawfulBEq
+
+def hash (dt : DataType) (x : dt.toType) : UInt64 :=
+  match dt with
+  | bool => Hashable.hash x
+  | nat => Hashable.hash x
+  | string => Hashable.hash x
+  | option dt =>
+    -- Taken from Init.Data
+    match x with
+    | none => 11
+    | some x => mixHash (hash dt x) 13
+  | array dt =>
+    -- Taken from Init.Data
+    x.foldl (fun r a => mixHash r (hash dt a)) 7
+
+instance {dt : DataType} : Hashable dt.toType where
+  hash := hash dt
+
 end DataType
 
 end Tables
+
+end
